additions to the framework and red black trees case study

examples/RedBlack/testing.v
@@ -1,5 +1,6 @@
 Require Import QuickChick.
-Require Import SetOfOutcomes EndToEnd.
+Require Import ModuleGen GenCombinators.
+Import Gen GenComb.
 Require Import NPeano.
 
 Require Import ssreflect ssrnat ssrbool eqtype.
@@ -36,16 +37,31 @@ Fixpoint black_height_bool (t: tree) : option nat :=
 Definition is_black_balanced (t : tree) : bool :=
   isSome (black_height_bool t).
 
-Fixpoint has_no_red_red (t : tree) : bool :=
+Fixpoint has_no_red_red (c : color) (t : tree) : bool :=
   match t with
-  | Leaf => true
-  | Node Red (Node Red _ _ _) _ _ => false
-  | Node Red _ _ (Node Red _ _ _) => false
-  | Node _ tl _ tr => has_no_red_red tl && has_no_red_red tr
+    | Leaf => true
+    | Node Red t1 _ t2 => 
+      match c with 
+        | Red => false 
+        | Black => has_no_red_red Red t1 && has_no_red_red Red t2
+      end
+    | Node Black t1 _ t2 => 
+      has_no_red_red Black t1 && has_no_red_red Black t2
   end.
 
-Definition is_redblack_bool (t : tree) : bool  :=
-  is_black_balanced t && has_no_red_red t.
+Definition has_parent (c : color) (t: tree) : bool :=
+  match t with
+    | Leaf => true
+    | Node Black _ _ _ => true
+    | Node Red _ _ _ => 
+      match c with 
+        | Black => true 
+        | _ => false
+      end
+  end.
+
+Definition is_redblack_bool (t : tree) : bool := 
+  is_black_balanced t && has_no_red_red Red t.
 
 Fixpoint showColor (c : color) :=
   match c with
@@ -67,22 +83,16 @@ Instance showTree {A : Type} `{_ : Show A} : Show tree :=
     show t := "" (* CH: tree_to_string t causes a 9x increase in runtime *)
   |}.
 
-Section Checker.
-  Context {Gen : Type -> Type}
-          {H: GenMonad Gen}.
+Definition insert_is_redblack_checker (genTree : G tree) : Checker :=
+  forAll arbitraryNat (fun n =>
+  (forAll genTree (fun t =>
+  (is_redblack_bool t ==>
+   is_redblack_bool (insert n t))))).
 
-  Variable genTree : Gen tree.
+Definition genColor := elements Red [Red; Black].
 
-  Definition insert_is_redblack_checker : Gen QProp :=
-    forAll arbitraryNat (fun n =>
-    (forAll genTree (fun t =>
-      (is_redblack_bool t ==>
-       is_redblack_bool (insert n t)) : Gen QProp)) : Gen QProp).
-
-  Definition genColor := elements Red [Red; Black].
-
-  Fixpoint genAnyTree_max_height (h : nat) : Gen tree :=
-    match h with 
+Fixpoint genAnyTree_max_height (h : nat) : G tree :=
+  match h with 
     | 0 => returnGen Leaf
     | S h' =>
         bindGen genColor (fun c =>
@@ -92,9 +102,7 @@ Section Checker.
         returnGen (Node c t1 n t2)))))
     end.
 
-  Definition genAnyTree : Gen tree := sized genAnyTree_max_height.
-
-End Checker.
+Definition genAnyTree : G tree := sized genAnyTree_max_height.
 
 Definition testInsertNaive :=
   showResult (quickCheck (insert_is_redblack_checker genAnyTree)).
@@ -104,18 +112,14 @@ Extract Constant Test.defNumTests => "10".
 QuickCheck testInsertNaive.
 Extract Constant Test.defNumTests => "10000".
 
-Section Generators.
-  Context {Gen : Type -> Type}
-          {H: GenMonad Gen}.
-
-  Fixpoint genRBTree_height (h : nat) (c : color) :=
-    match h with
-      | 0 =>
-        match c with
-          | Red => returnGen Leaf
-          | Black => oneof (returnGen Leaf)
-                           [returnGen Leaf;
-                             bindGen arbitraryNat (fun n =>
+Fixpoint genRBTree_height (h : nat) (c : color) :=
+  match h with
+    | 0 =>
+      match c with
+        | Red => returnGen Leaf
+        | Black => oneof (returnGen Leaf)
+                         [returnGen Leaf;
+                           bindGen arbitraryNat (fun n =>
                              returnGen (Node Red Leaf n Leaf))]
         end
       | S h =>
@@ -147,9 +151,8 @@ Section Generators.
         end
     end.
 
-  Definition genRBTree := sized (fun h => genRBTree_height h Red).
-
-End Generators.
+Definition genRBTree := 
+  bindGen arbitrary (fun h => genRBTree_height h Red).
 
 Definition showDiscards (r : Result) :=
   match r with
