examples/RedBlack/verif.v
@@ -1,119 +1,269 @@
 Require Import ssreflect ssrnat ssrbool eqtype.
-
 Require Import List String.
-
 Require Import QuickChick.
-Require Import SetOfOutcomes EndToEnd.
+Import Gen GenComb.
 
 Require Import redblack.
 Require Import testing.
+
+Lemma has_black_height :
+  forall t h c, is_redblack' t c h -> black_height_bool t = Some h.
+Proof.
+  elim => [| c t1 IHt1 n t2 IHt2] h c' Hrb; first by inversion Hrb. 
+  inversion Hrb as [| n' tl tr h' Htl Htr | c'' n' tl tr h' Htl Htr]; subst;
+  move: Htl Htr => /IHt1 Htl /IHt2 Htr; simpl; by rewrite Htl Htr eq_refl.  
+Qed.
+ 
+Lemma is_redblack'P :
+  forall (t : tree) n c,
+    reflect (is_redblack' t c n)
+            ((black_height_bool t == Some n) && has_no_red_red c t).
+Proof.
+  elim => [| c t1 IHt1 n t2 IHt2] n' c'. 
+  - simpl.
+    apply (@iffP ((Some 0 == Some n') && true));
+    first by apply/idP.
+    + move => /andP [/eqP [H1] _]; subst. 
+      econstructor.
+    + move => Hrb. apply/andP. inversion Hrb; subst. split => //.
+  - apply (@iffP ((black_height_bool (Node c t1 n t2) == Some n') &&
+                   has_no_red_red c' (Node c t1 n t2)));
+    first by apply/idP.
+    + move => /andP [/eqP H1 H2]; subst. simpl in H1, H2.
+      remember (black_height_bool t1) as h1.
+      remember (black_height_bool t2) as h2. 
+      destruct h1, h2; (try discriminate).
+      have Heq : (n0 = n1) by apply/eqP; destruct (n0 == n1). subst.
+      rewrite eq_refl in H1. 
+      destruct c; inversion H1; subst; clear H1;
+      destruct c' => //=; move : H2 => /andP [Ht1 Ht2]; 
+      (constructor; [apply/IHt1 | apply/IHt2]); apply/andP; split => //.
+    + move => Hrb. 
+      inversion Hrb as [| n'' tl tr h Hrbl Hrbr | c'' n'' tl tr h Hrbl Hrbr]; subst;
+      move: Hrbl Hrbr => /IHt1/andP [/eqP Hbhl Hrrl] /IHt2/andP [/eqP Hbhr Hrrr];
+      apply/andP; split => //; simpl; (try by rewrite Hbhl Hbhr eq_refl);
+      by (apply/andP; split => //).
+Qed.
 
 Lemma is_redblackP :
   forall (t : tree),
     reflect (is_redblack t) (is_redblack_bool t).
 Proof.
-  move => t. induction t.
-  - constructor. rewrite /is_redblack. exists 0. by constructor.
-  - admit.
-Admitted. (* TODO *)
+  move => t. 
+  apply (@iffP (is_redblack_bool t)); first by apply/idP.
+  rewrite /is_redblack_bool.
+  + move => /andP [Hb Hrr]. rewrite /is_black_balanced in Hb.
+    have [h Hbh] : exists h, black_height_bool t = Some h
+      by destruct (black_height_bool t) => //; eexists.
+    exists h. apply/is_redblack'P. apply/andP; split => //; apply/eqP => //.
+  + move => [h /is_redblack'P /andP [/eqP H1 H2]]. 
+    rewrite /is_redblack_bool /is_black_balanced H1. apply/andP; split => //.
+Qed.
 
 Lemma genColor_correct:
-  genColor <--> all.
+  semGen genColor <--> fun _ => True.
 Proof.
-  rewrite /genColor. intros c. rewrite elements_equiv.
+  rewrite /genColor. intros c. rewrite semElements.
   split => // _. left.
   destruct c;  by [ constructor | constructor(constructor)].
 Qed.
 
-(* ugly proof, needs refactoring at some point *)
-Lemma genRBTree_height_correct:
-  forall c h,
-    (genRBTree_height h c) <--> (fun t => is_redblack' t c h).
+Lemma genColor_correctSize:
+  forall s,
+    semSize genColor s <--> fun _ => True.
 Proof.
-  move => c h. move : c. induction h as [| h]; intros c' t.
-  { rewrite /genRBTree_height. split.
-    - destruct c'.
-      + rewrite returnGen_def. by move => <-; constructor.
-      + rewrite oneof_equiv. move => [[gen [H Hgen]] | [// H Hret]].
-        inversion H as [HIn | HIn]; subst.
-        * rewrite returnGen_def in Hgen; subst. by constructor.
-        * inversion HIn as [HIn' |  HIn'] => //; subst.
-        move: Hgen => [n [Hn Hret]]. rewrite returnGen_def in Hret; subst.
-          by constructor; constructor.
-    - move=> H. inversion H; subst.
-      + destruct c' => //. rewrite oneof_equiv. left.
-        eexists. by split; [by apply in_eq |].
-      + rewrite oneof_equiv. left. eexists.
-        split. by constructor(apply in_eq).
-        eexists. split; first by apply arbNat_correct.
-        inversion H0; subst. inversion H1; subst.
-        reflexivity. }
-  { split.
-    - destruct c'.
-      + move => [tl [/IHh Hgentl [tr [/IHh Hgentr [n [_ H]]]]]].
-        rewrite returnGen_def in H; subst.
-        by constructor => //.
-      + move => [[] [Hcol Hgen]].
-        * move : Hgen =>
-          [tl1 [/IHh Htl1 [tl2 [/IHh Htl2 [tr1 [/IHh Htr1 [tr2 [/IHh Htr2 H]]]]]]]].
-          move : H => [n [_ [nl [_ [nr [_ H]]]]]].
-          rewrite returnGen_def in H; subst.
-          constructor; constructor=> //.
-       * move : Hgen => [tl [/IHh Hgentl [tr [/IHh Hgentr [n [_ H]]]]]].
-         rewrite returnGen_def in H; subst.
-         constructor => //.
-    - move => H. inversion H as [| n tl tr h' Hrbl Hrbr |
-                                   c n tl tr h' Hrbl Hrbr]; subst.
-      + inversion Hrbl as [| |c n1 tl1 tr1 h1 Hrbl1 Hrbr1]; subst.
-        inversion Hrbr as [| |c n2 tl2 tr2 h2 Hrbl2 Hrbr2]; subst.
-        exists Red. split; first by apply genColor_correct.
-        exists tl1. split; first by apply IHh.
-        exists tl2. split; first by apply IHh.
-        exists tr1. split; first by apply IHh.
-        exists tr2. split; first by apply IHh.
-        exists n. split; first by apply arbNat_correct.
-        exists n1. split; first by apply arbNat_correct.
-        exists n2. split; first by apply arbNat_correct.
-        reflexivity.
-      + destruct c'.
-        * exists tl. split; first by apply IHh.
-          exists tr. split; first by apply IHh.
-          exists n. split; first by apply arbNat_correct.
-          reflexivity.
-        * exists Black. split; first by apply genColor_correct.
-          exists tl. split; first by apply IHh.
-          exists tr. split; first by apply IHh.
-          exists n. split; first by apply arbNat_correct.
-          reflexivity. }
+  rewrite /genColor. intros s c.
+  split => // _. apply semElementsSize. left.
+  destruct c; by [ constructor | constructor(constructor)].
 Qed.
 
-Lemma genRBTree_correct:
-  genRBTree <--> is_redblack.
+  Axiom semOneofSize:
+    forall {A} (l : list (G A)) (def : G A) s,
+      (semSize (oneof def l) s) <-->
+      (fun e => (exists x, List.In x l /\ semSize x s e) \/ 
+                (l = nil /\ semSize def s e)).
+
+
+(* Some helpful lemmas and definitions *)
+
+Inductive all_nodes_bellow (s : nat) : tree -> Prop :=
+| Bellow_l : all_nodes_bellow s Leaf
+| Bellow_N : 
+    forall c t1 n t2, 
+      all_nodes_bellow s t1 ->
+      all_nodes_bellow s t2 ->
+      (n <= s)%coq_nat ->
+      all_nodes_bellow s (Node c t1 n t2).
+
+Definition max_node : tree -> nat -> nat :=
+  fix f t m :=
+  match t with
+    | Leaf => m
+    | Node _ t1 n t2 =>
+      max (f t1 (max m n)) (f t2 (max m n))
+  end. 
+
+
+Lemma all_nodes_bellow_greater :
+  forall m n t, 
+    n <= m ->
+    all_nodes_bellow n t ->
+    all_nodes_bellow m t.
 Proof.
-  move => t. split.
-  - rewrite /genRBTree sized_def.
-    move => [n /genRBTree_height_correct Hgen].
-    eexists. eassumption.
-  - rewrite /is_redblack. move => [h /genRBTree_height_correct  Hgen].
-    rewrite /genRBTree sized_def. by exists h.
+  move => m n t. 
+  elim : t m n => [| c tl IHtl nd tr IHtr] m n Hleq Hb; try by constructor.
+  inversion Hb; subst; constructor; eauto. 
+  eapply Le.le_trans; eauto. by apply/leP.
+Qed.
+
+Lemma max_node_less:
+  forall t n, 
+    (n <= max_node t n)%coq_nat.
+Proof.
+    elim => [| /= c tl IHtl nd tr IHtr] n; auto. 
+    apply Max.max_case_strong =>  Hcmp; auto;
+    apply Max.max_case_strong =>  Hcmp'; auto;
+    eapply Le.le_trans; try eassumption;
+    [apply IHtl | apply IHtr].
+Qed.
+
+(* ugly proof, needs refactoring at some point *)
+
+Lemma genRBTree_height_correct:
+  forall c h s,
+    semSize (genRBTree_height h c) s <--> 
+    (fun t => is_redblack' t c h /\ all_nodes_bellow s t).
+Proof.
+  move => c h s. move : c s. induction h as [| h IHh]; intros c' s t.
+  { rewrite /genRBTree_height. split.
+    - destruct c'.
+      + rewrite semReturnSize. by move => <-; split; constructor.
+      + rewrite semOneofSize.  move => [[gen [H Hgen]] | [// H Hret]].
+        inversion H as [HIn | HIn]; subst.
+        * apply semReturnSize in Hgen; subst. split; by constructor.
+        * inversion HIn as [HIn' |  HIn'] => //; subst.
+          move: Hgen => /semBindSize [a [Hsize1 /semReturnSize Heq]]; subst. 
+          split; try by constructor(constructor). 
+          constructor; try by constructor. by apply arbNat_correctSize.
+    - move=> [Hsize Hbellow]. inversion Hsize; subst.
+      + destruct c'; first by apply semReturnSize. rewrite semOneofSize. left.
+        eexists. split; [by apply in_eq | by apply semReturnSize].
+      + rewrite semOneofSize. left. eexists.
+        split. by constructor(apply in_eq).
+        apply semBindSize. simpl in *.
+        inversion H; inversion H0; inversion Hbellow; subst.
+        exists n; split; first by apply arbNat_correctSize; auto.
+        by apply semReturnSize. }
+  { split.
+    - move => /= Hsize.  destruct c'.
+      + move: Hsize => /semBindSize [t' [Hsize 
+                       /semBindSize [t1 [Hsize1
+                       /semBindSize [t2 [/arbNat_correctSize Hnat 
+                                         /semReturnSize Heq]]]]]]; subst.
+        move : Hsize Hsize1 => /IHh [Hrb Hbellow] /IHh [Hrb1 Hbellow1].
+        split; constructor; eassumption.
+      + move : Hsize => /semBindSize [c [_ Hsize]]. 
+        destruct c.
+        * move : Hsize => /semBindSize [tl1 [/IHh [Hrbl1 Hbl1] 
+                          /semBindSize [tl2 [/IHh [Hrbl2 Hbl2]
+                          /semBindSize [tr1 [/IHh [Hrbr1 Hbr1]
+                         /semBindSize [tr2 [/IHh [Hrbr2 Hbr2]
+                         /semBindSize [n [/arbNat_correctSize Hn
+                         /semBindSize [nl [/arbNat_correctSize Hnl
+                         /semBindSize [nr [/arbNat_correctSize Hnr 
+                                           /semReturnSize Heq]]]]]]]]]]]]]];
+            subst; split; constructor; try constructor; try eassumption.
+        * move : Hsize => /semBindSize [t' [/IHh [Hrb Hb] 
+                          /semBindSize [t1 [/IHh [Hrb1 Hb1] 
+                          /semBindSize [t2 [/arbNat_correctSize Hn
+                                            /semReturnSize Heq]]]]]]; subst.
+          constructor; constructor; try eassumption.
+     - move => H. inversion H as [Hsize Hb]; clear H;
+       inversion Hsize as [| n tl tr h' Hrbl Hrbr |
+                           c n tl tr h' Hrbl Hrbr]; subst;
+       inversion Hb as [ |c t1 ? t2 Hbt1 Hbt2]; subst; clear Hb.
+       + inversion Hrbl as [| |c n1 tl1 tr1 h1 Hrbl1 Hrbr1]; subst.
+         inversion Hrbr as [| |c n2 tl2 tr2 h2 Hrbl2 Hrbr2]; subst.
+         inversion Hbt1 as [ | c t1 ? t2 Hbt11 Hbt12]; subst; clear Hbt1.
+         inversion Hbt2 as [ | c t1 ? t2 Hbt21 Hbt22]; subst; clear Hbt2.
+         simpl. apply semBindSize.
+         exists Red. split; first (by apply genColor_correctSize);
+         apply semBindSize. exists tl1. split; first by apply IHh.
+         apply semBindSize. exists tl2. split; first by apply IHh.
+         apply semBindSize. exists tr1. split; first by apply IHh.
+         apply semBindSize. exists tr2. split; first by apply IHh.
+         apply semBindSize. exists n. split; first by apply arbNat_correctSize.
+         apply semBindSize. exists n1. split; first by apply arbNat_correctSize.
+         apply semBindSize. exists n2. split; first by apply arbNat_correctSize.
+         apply semReturnSize; reflexivity.
+       + destruct c'. simpl.
+        * apply semBindSize. exists tl. split; first by apply IHh.
+          apply semBindSize. exists tr. split; first by apply IHh.
+          apply semBindSize. exists n. split; first by apply arbNat_correctSize.
+          apply semReturnSize; reflexivity.
+        * simpl. apply semBindSize. exists Black. 
+          split; first by apply genColor_correctSize.
+          apply semBindSize. exists tl. split; first by apply IHh.
+          apply semBindSize. exists tr. split; first by apply IHh.
+          apply semBindSize. exists n. split; first by apply arbNat_correctSize.
+          apply semReturnSize; reflexivity. }
+Qed.
+
+ 
+Lemma genRBTreeSize_correct:
+  forall s,
+    semSize genRBTree s <--> 
+    (fun t => 
+       (exists n, n <= s /\ is_redblack' t Red n) /\ 
+       all_nodes_bellow s t).
+Proof.
+  move => s t. rewrite /genRBTree /is_redblack. split.
+  - move => /semBindSize [n [/arbNat_correctSize /leP Hle 
+                             /genRBTree_height_correct [Hrb Hb]]].
+    split => //. exists n; split => //.
+  - move => [[n [Hle Hrb]] Hb].
+    apply semBindSize. exists n. 
+    split; first by apply arbNat_correctSize; apply/leP.
+    apply genRBTree_height_correct. split => //.
+Qed.
+
+Lemma all_nodes_bellow_max_node :
+  forall t n, 
+    all_nodes_bellow (max_node t n) t.
+Proof.
+  elim => [| c tl IHtl nd tr IHtr] n; try by constructor. 
+  constructor; simpl; 
+  try (apply Max.max_case_strong => /leP Hcmp; auto; 
+       eapply all_nodes_bellow_greater; try eassumption; auto).
+  apply (Max.max_case_strong n nd) => Hcmp; eauto;
+  [ eapply Le.le_trans; try eassumption |];
+  apply (Max.max_case_strong) => Hcmp'; apply max_node_less.
 Qed.
 
 Lemma insert_is_redblack_checker_correct:
-  semChecker (insert_is_redblack_checker genRBTree) <-> insert_preserves_redblack.
+  (forall s, 
+     semCheckerSize (insert_is_redblack_checker genRBTree) s) <-> 
+  insert_preserves_redblack.
 Proof.
-  rewrite /insert_is_redblack_checker /insert_preserves_redblack semForAll.
+  rewrite /insert_is_redblack_checker /insert_preserves_redblack. 
   split.
-  + move => H x s Hrb.
-    have /H/semPredQProp/semForAll H' : @arbitraryNat Pred _ x
-      by apply arbNat_correct.
-    have /H'/semPredQProp/semImplication H'': @genRBTree Pred _ s
-      by apply genRBTree_correct.
-    apply/is_redblackP.
-    by move/is_redblackP/H''/semBool: Hrb.
-  + move=> H a _.
-    apply/semPredQProp/semForAll. move => t Hgen.
-    apply/semPredQProp/semImplication. move => Hrb.
-    apply/semBool. apply/is_redblackP.
-    move: Hrb => /is_redblackP [n Hrb]. eapply H.
-    eexists. eassumption.
+  - move => H x t [n' Hrb]. set s := max (max_node t x) n'.
+    move : H => /(_ s) /semForAll H.
+    have /H/semPredQProp/semForAll Hx : semSize arbitraryNat s x.
+    { apply arbNat_correctSize. 
+      apply Le.le_trans with (m := (max_node t x)). 
+      apply max_node_less. rewrite /s. apply Max.le_max_l. }
+    have /Hx/semPredQProp/semImplication Ht : semSize genRBTree s t.
+    { apply genRBTreeSize_correct. split. 
+      - exists n'. split => //. rewrite /s. apply/leP. apply Max.le_max_r.
+      - rewrite /s. apply Max.max_case_strong => Hcmp; eauto;
+        [| apply all_nodes_bellow_greater with (n := max_node t x); 
+           try by apply/leP]; apply all_nodes_bellow_max_node. }
+    have /is_redblackP/Ht/semBool Hins : is_redblack t by exists n'.
+    by apply/is_redblackP.
+  - move => H s. apply semForAll => n /arbNat_correctSize Hle.
+    apply semPredQProp. 
+    apply semForAll => t /genRBTreeSize_correct [[n' [Hle' Hrb]] Hb].
+    apply semPredQProp. apply semImplication => /is_redblackP Hbool.
+    apply semBool. apply/is_redblackP. by eapply H.
 Qed.
