src/Arbitrary.v
@@ -3,7 +3,7 @@ Require Import ZArith ZArith.Znat Arith.
 Require Import Coq.Numbers.Natural.Peano.NPeano.
 Require Import Recdef.
 Require Import List.
-Require Import ssreflect.
+Require Import ssreflect ssrbool ssrnat.
 
 Import Gen GenComb.
 Class Arbitrary (A : Type) : Type :=
@@ -38,7 +38,7 @@ Function shrinkNat (x : nat) {measure (fun x => x) x}: list nat :=
   end.
 Proof.
   intros; simpl; pose proof (divmod_spec n 1 0 0).
-  assert (H01 : 0 <= 1) by omega; apply H in H01; subst; clear H.
+  assert (H01 : (0 <= 1)%coq_nat) by omega; apply H in H01; subst; clear H.
   destruct (divmod n 1 0 0); destruct n1; simpl; omega.
 Qed.
 
@@ -115,19 +115,56 @@ Lemma arbNat_correct:
 Proof.
   rewrite /arbitrary /arbNat /arbitraryNat. move => n.
   split => // _.
-  apply semSizedSize. exists n. apply semChooseSize.
+  apply semSized. exists n. apply semChooseSize.
   split=> //.
 Qed.
 
+
 Lemma arbInt_correct:
+  forall s,
+    semSize arbitrary s <--> 
+    (fun (z : Z) =>  (- Z.of_nat s <= z <= Z.of_nat s)%Z).
+Proof.
+  rewrite /arbitrary /arbInt /arbitraryZ. move => n. split.
+  - move/semSizedSize/semChooseSize => /= [H1 H2].
+    split; by apply Zle_bool_imp_le.
+  - move => [H1 H2].
+    apply semSizedSize. apply semChooseSize.
+    split; by apply Zle_imp_le_bool. 
+Qed.
+
+
+Lemma arbBool_correctSize:
+  forall s,
+    semSize arbitrary s <--> (fun (_ : bool) => True).
+Proof.
+  rewrite /arbitrary /arbBool /arbitraryBool. move => b.
+  split => // _. apply semChooseSize. 
+  case: b; case: a; split => //=. 
+Qed.
+
+Lemma arbNat_correctSize:
+  forall s, 
+    semSize arbitrary s <--> (fun (n : nat) => (n <= s)%coq_nat).
+Proof.
+  rewrite /arbitrary /arbNat /arbitraryNat. move => n.
+  split.
+  - by move/semSizedSize/semChooseSize => /= [H1 /leP H2]. 
+  - move => /leP H.
+    apply semSizedSize. apply semChooseSize.
+    split; auto. 
+Qed.
+
+Lemma arbInt_correctSize:
   semGen arbitrary <--> (fun (_ : Z) => True).
 Proof.
   rewrite /arbitrary /arbInt /arbitraryZ. move => n. split => // _.
-  apply semSizedSize.
+  apply semSized.
   exists (Z.abs_nat n). apply semChooseSize.
   by split => //=; rewrite Nat2Z.inj_abs_nat; 
      case: n => //= p; apply Z.leb_refl.
 Qed.
+
 
 (* TODO : this need semListOf *)
 Lemma arbList_correct:
