src/QuickChick.v
@@ -1,12 +1,13 @@
 Declare ML Module "quickChick".
 
 Require Export Show.
-
 Require Export Axioms.
 Require Export ModuleGen.
 Require Export GenCombinators.
 Require Export Arbitrary.
 Require Export State.
 Require Export Checker.
+Require Export SemChecker.
 Require Export Test.
 Require Export Extraction.
+
